[OLty] Semantic types: binding-related properties
- Require them to hold only for closed values.
- Implement substitution by precomposition and related properties.

theories/olty.v
@@ -3,12 +3,11 @@ From D Require Import iris_prelude asubst_base asubst_intf dlang.
 From iris.proofmode Require Import tactics.
 From iris.program_logic Require Import language.
 From D.pure_program_logic Require Import lifting adequacy.
-From D Require Export gen_iheap saved_interp.
 
-Module Type OLty (Import VS: VlSortsSig).
+From Coq Require ProofIrrelevance FunctionalExtensionality.
 
-(* Instead of duplicating [envD], Include LiftWp: *)
-(* Notation envD Σ := (vls -d> vl -d> iProp Σ). *)
+Module Type OLty (Import VS: VlSortsFullSig).
+
 Include LiftWp VS.
 
 Section olty_limit_preserving.
@@ -16,10 +15,25 @@ Section olty_limit_preserving.
 
   Definition envD_persistent (A : envD Σ) := ∀ ρ w, Persistent (A ρ w).
 
-  Global Instance: LimitPreserving envD_persistent.
+  Instance: LimitPreserving envD_persistent.
   Proof.
     apply limit_preserving_forall=> ρ; apply limit_preserving_forall=> w.
       apply bi.limit_preserving_Persistent => n ?? H. exact: H.
+  Qed.
+
+  Definition vclosed (A : envD Σ) := ∀ ρ v, A ρ v ⊢ ⌜ nclosed_vl v 0 ⌝.
+
+  Instance: LimitPreserving vclosed.
+  Proof.
+    apply limit_preserving_forall=> ρ; apply limit_preserving_forall=> w.
+    apply limit_preserving_entails; last apply _.
+    solve_proper_ho.
+  Qed.
+
+  Definition restrict A := vclosed A ∧ envD_persistent A.
+  Global Instance: LimitPreserving restrict.
+  Proof.
+    apply limit_preserving_and; apply _.
   Qed.
 End olty_limit_preserving.
 
@@ -29,10 +43,12 @@ and values. Adapted from
 https://gitlab.mpi-sws.org/iris/examples/blob/d4f4153920ea82617c7222aeeb00b6710d51ee03/theories/logrel_heaplang/ltyping.v#L5. *)
 Record olty Σ := Olty {
   olty_car : envD Σ;
-  olty_persistent ρ v : Persistent (olty_car ρ v)
+  olty_v_closed : vclosed olty_car;
+  olty_persistent ρ v : Persistent (olty_car ρ v);
 }.
-Arguments Olty {_} _%I {_}.
+Arguments Olty {_} _%I _ {_}.
 Arguments olty_car {_} _ _ _ /.
+Arguments olty_v_closed {_} _ _ _ /.
 Bind Scope olty_scope with olty.
 Delimit Scope olty_scope with T.
 Existing Instance olty_persistent.
@@ -55,35 +71,204 @@ Section olty_ofe.
   (* Only needed to define Olty using Iris fixpoints (e.g. for normal recursive types). *)
   Global Instance olty_cofe : Cofe oltyC.
   Proof.
-    apply (iso_cofe_subtype' envD_persistent
-      (@Olty _) olty_car)=> //; rewrite /envD_persistent; apply _.
+    set curry_olty : ∀ A, restrict A → olty Σ := λ A '(conj P1 P2), @Olty Σ A P1 P2.
+    apply (iso_cofe_subtype' restrict curry_olty olty_car) => //.
+    - by move => [].
+    - by move => ? [].
+    - apply _.
   Qed.
 
-  Global Program Instance olty_inhabited : Inhabited (olty Σ) := populate (Olty (λ _ _, False)%I).
+  Global Program Instance olty_inhabited : Inhabited (olty Σ) := populate (Olty (λ _ _, False)%I _).
+  Next Obligation. by unseal=>?. Qed.
 
   Global Instance olty_car_ne: NonExpansive (@olty_car Σ).
   Proof. by intros ??. Qed.
   Global Instance lty_car_proper : Proper ((≡) ==> (≡)) (@olty_car Σ).
   Proof. apply ne_proper, olty_car_ne. Qed.
 
-  Definition pack φ : olty Σ := Olty (λ ρ v, □ φ ρ v)%I.
+  Program Definition pack φ (Hvc : vclosed φ) := Olty (λ ρ v, □ φ ρ v)%I _.
+  Next Obligation. rewrite /vclosed; intros. iIntros "?". by iApply Hvc. Qed.
+
   Lemma persistently_id (P : iProp Σ) `{!Persistent P}: □P ⊣⊢ P.
   (* Proof. by iSplit; iIntros. Qed. *)
   Proof. apply: intuitionistic_intuitionistically. Qed.
 
-  Lemma olty_car_pack_id φ `{∀ ρ v, Persistent (φ ρ v)} :
-    olty_car (pack φ) ≡ φ.
+  Lemma olty_car_pack_id φ (H : vclosed φ) `{∀ ρ v, Persistent (φ ρ v)} :
+    olty_car (pack φ H) ≡ φ.
   Proof.
     move => ?? /=.
     apply: intuitionistic_intuitionistically.
   Qed.
 
-  Lemma pack_olty_car_id τ : pack (olty_car τ) ≡ τ.
+  Lemma pack_olty_car_id τ : pack (olty_car τ) (olty_v_closed τ) ≡ τ.
   Proof.
-    move: τ => []????/=.
+    move: τ => []?????/=.
     apply: intuitionistic_intuitionistically.
   Qed.
+
+  Global Instance ids_envD : Ids (envD Σ) := λ _, inhabitant.
+  Global Instance rename_envD : Rename (envD Σ) :=
+    λ r φ ρ, φ (r >>> ρ).
+  Global Instance hsubst_envD : HSubst vl (envD Σ) :=
+    λ sb φ ρ, φ (sb >> ρ).
+
+  Ltac renLemmas_envD :=
+    hnf; rewrite /hsubst /hsubst_envD => /= *;
+    try (apply FunctionalExtensionality.functional_extensionality_dep => ?); by asimpl.
+
+  Global Instance HSubstLemmas_envD : HSubstLemmas vl (envD Σ).
+  Proof. split => //; renLemmas_envD. Qed.
+
+  (*
+    Since substitution lemmas don't use setoids,
+    [HSubstLemmas vl (olty Σ)] requires proof irrelevance.
+   *)
+
+  Lemma olty_eq τ1 τ2: olty_car τ1 = olty_car τ2 → τ1 = τ2.
+  Proof.
+    move: τ1 τ2 => [φ1 ??] [φ2 ??]; rewrite /olty_car.
+    destruct 1. f_equal; exact: ProofIrrelevance.proof_irrelevance.
+  Qed.
+
+  Global Instance ids_olty : Ids (olty Σ) := λ _, inhabitant.
+  Global Program Instance rename_olty : Rename (olty Σ) :=
+    λ r τ, Olty (rename r (olty_car τ)) _.
+  Next Obligation. rewrite /vclosed; intros. exact: olty_v_closed. Qed.
+  Global Program Instance hsubst_olty : HSubst vl (olty Σ) :=
+    λ sb τ, Olty ((olty_car τ).|[sb]) (_ (olty_car τ).|[sb]).
+  Next Obligation. rewrite /vclosed; intros. exact: olty_v_closed. Qed.
+
+  Global Instance hsubstLemmas_olty : HSubstLemmas vl (olty Σ).
+  Proof.
+    split=> [s|??|?? s]; apply olty_eq => //; case: s => [φ??];
+    rewrite /hsubst /hsubst_olty /olty_car.
+    all: trivial using hsubst_id, id_hsubst, hsubst_comp.
+  Qed.
+
+(* Global Instance rename_olty2 : Rename (olty Σ) :=
+    λ r τ, Olty (λ ρ, τ (r >>> ρ)) (λ ρ, olty_v_closed τ _).
+  Global Instance hsubst_olty2 : HSubst vl (olty Σ) :=
+    λ sb τ, Olty (λ ρ, τ (sb >> ρ)) (λ ρ, olty_v_closed τ _).
+  Global Instance HSubstLemmas_olty2 : HSubstLemmas vl (olty Σ).
+  Proof.
+    split=> [s|??|?? s]; apply olty_eq => //; case: s => [φ??];
+    (apply functional_extensionality_dep => ?);
+    rewrite /hsubst /hsubst_olty2 /olty_car /=.
+    all: by asimpl.
+  Qed. *)
+
+  Lemma envD_weaken ρ1 ρ2 ρ3 φ :
+    φ.|[upn (length ρ1) (ren (+ length ρ2))] (to_subst (ρ1 ++ ρ2 ++ ρ3))
+    = φ (to_subst (ρ1 ++ ρ3)).
+  Proof. rewrite /hsubst_envD /hsubst to_subst_weaken //. Qed.
+
+  Lemma envD_subst_up ρ1 ρ2 v φ :
+    φ.|[upn (length ρ1) (v.[ren (+length ρ2)] .: ids)] (to_subst (ρ1 ++ ρ2))
+    ≡ φ (to_subst (ρ1 ++ v :: ρ2)).
+  Proof. rewrite /hsubst_envD /hsubst to_subst_up //. Qed.
+
+  Lemma olty_weaken ρ1 ρ2 ρ3 τ :
+    τ.|[upn (length ρ1) (ren (+ length ρ2))] (to_subst (ρ1 ++ ρ2 ++ ρ3))
+    = τ (to_subst (ρ1 ++ ρ3)).
+  Proof.
+    (* rewrite /hsubst_olty /hsubst_envD /hsubst /= to_subst_weaken //. *)
+    rewrite [@hsubst _ _ hsubst_olty]/hsubst /hsubst_olty /=.
+    exact: envD_weaken.
+  Qed.
+
+  Lemma olty_subst_up ρ1 ρ2 v τ :
+    τ.|[upn (length ρ1) (v.[ren (+length ρ2)] .: ids)] (to_subst (ρ1 ++ ρ2))
+    ≡ τ (to_subst (ρ1 ++ v :: ρ2)).
+  Proof.
+    (* rewrite /hsubst_olty /hsubst_envD /hsubst /= to_subst_up //. *)
+    rewrite [@hsubst _ _ hsubst_olty]/hsubst /hsubst_olty /=.
+    exact: envD_subst_up.
+  Qed.
+
+  Definition sCtx := list (olty Σ).
+
+  Fixpoint env_oltyped (Γ : sCtx) (ρ : var → vl) : iProp Σ :=
+    match Γ with
+    | φ :: Γ' => env_oltyped Γ' ((+1) >>> ρ) ∗ φ ρ (ρ 0)
+    | nil => True
+    end%I.
+
+  Global Instance env_oltyped_persistent (Γ : sCtx) vs: Persistent (env_oltyped Γ vs).
+  Proof. elim: Γ vs => [|τ Γ IHΓ] vs /=; apply _. Qed.
+
+  Lemma env_oltyped_cl_ρ Γ ρ :
+    env_oltyped Γ ρ -∗ ⌜ nclosed_sub (length Γ) 0 ρ ⌝.
+  Proof.
+    elim: Γ ρ => [|φ Γ IHΓ] ρ /=; [| rewrite IHΓ /olty2fun olty_v_closed ]; iIntros "!% //".
+    - move => [Hclρ Hclp0] [|i /lt_S_n] Hle. exact Hclp0. apply Hclρ, Hle.
+  Qed.
+
+  Lemma env_oltyped_cl_app `{Sort X} (x : X) Γ ρ:
+    env_oltyped Γ ρ -∗
+    ⌜ nclosed x (length Γ) ⌝ → ⌜ nclosed x.|[ρ] 0 ⌝.
+  Proof. rewrite env_oltyped_cl_ρ. iIntros "!%". exact: nclosed_sub_app. Qed.
+
+  Lemma env_oltyped_cl_app_vl v Γ ρ:
+    env_oltyped Γ ρ -∗
+    ⌜ nclosed_vl v (length Γ) ⌝ → ⌜ nclosed_vl v.[ρ] 0 ⌝.
+  Proof. rewrite env_oltyped_cl_ρ. iIntros "!%". exact: nclosed_sub_app_vl. Qed.
+
+  Fixpoint env_oltyped_fin (Γ : sCtx) vs : iProp Σ :=
+    match Γ, vs with
+    | φ :: Γ', v :: vs => env_oltyped_fin Γ' vs ∗ φ (v .: to_subst vs) v
+    | nil, nil => True
+    | _, _ => False
+    end%I.
+  Notation "⟦ Γ ⟧*" := (env_oltyped_fin Γ).
+
+  Global Instance env_oltyped_fin_persistent (Γ : sCtx) vs: Persistent (⟦ Γ ⟧* vs).
+  Proof. elim: Γ vs => [|τ Γ IHΓ] [|v vs] /=; apply _. Qed.
+
+  Lemma env_oltyped_transl Γ vs :
+    ⟦ Γ ⟧* vs -∗ env_oltyped Γ (to_subst vs).
+  Proof.
+    elim: Γ vs => [|Γ φ IHΓ] [|v vs] /=;
+      by [|iIntros "[]"|asimpl; rewrite IHΓ].
+  Qed.
+
+  Lemma env_oltyped_fin_cl_ρ Γ ρ:
+    ⟦ Γ ⟧* ρ -∗ ⌜ nclosed_sub (length Γ) 0 (to_subst ρ) ⌝.
+  Proof. rewrite env_oltyped_transl env_oltyped_cl_ρ //. Qed.
+
+  Lemma env_oltyped_fin_cl_app `{Sort X} (x : X) Γ ρ:
+    ⟦ Γ ⟧* ρ -∗
+    ⌜ nclosed x (length Γ) ⌝ → ⌜ nclosed x.|[to_subst ρ] 0 ⌝.
+  Proof. rewrite env_oltyped_transl env_oltyped_cl_app //. Qed.
+
+  Lemma env_oltyped_fin_cl_app_vl v Γ ρ:
+    ⟦ Γ ⟧* ρ -∗
+    ⌜ nclosed_vl v (length Γ) ⌝ → ⌜ nclosed_vl v.[to_subst ρ] 0 ⌝.
+  Proof. rewrite env_oltyped_transl env_oltyped_cl_app_vl //. Qed.
+
+  Lemma interp_env_len_agree Γ ρ:
+    ⟦ Γ ⟧* ρ -∗ ⌜ length ρ = length Γ ⌝.
+  Proof.
+    elim: Γ ρ => [|τ Γ IHΓ] [|v ρ] //=; try by iPureIntro.
+    rewrite IHΓ. by iIntros "[-> _] !%".
+  Qed.
+
+  Lemma interp_env_ρ_closed Γ ρ: ⟦ Γ ⟧* ρ -∗ ⌜ cl_ρ ρ ⌝.
+  Proof.
+    elim: Γ ρ => [|τ Γ IHΓ] [|v ρ] //=; try by iPureIntro.
+    rewrite IHΓ /olty2fun olty_v_closed. iPureIntro. intuition.
+  Qed.
+
+  Lemma interp_env_props Γ ρ:
+    ⟦ Γ ⟧* ρ -∗ ⌜ cl_ρ ρ ∧ length ρ = length Γ ⌝.
+  Proof.
+    iIntros "#HG".
+    iDestruct (interp_env_ρ_closed with "HG") as %?.
+    iDestruct (interp_env_len_agree with "HG") as %?.
+    by iPureIntro.
+  Qed.
 End olty_ofe.
+
+Notation "⟦ Γ ⟧*" := (env_oltyped_fin Γ).
 Arguments oltyC : clear implicits.
 
 (* Different from normal TyInterp. Better? *)
